michael_formal/not4afp/Filesystem.thy
@@ -2,7 +2,7 @@ theory Filesystem
 imports "../Contexts" "../EFSM" "HOL-Library.Code_Target_Int"
 begin
 
-(* Takes a user ID and stores it in r1 *)
+\<comment> \<open> Takes a user ID and stores it in r1 \<close>
 definition login :: "transition" where
 "login \<equiv> \<lparr>
         Label = ''login'',
@@ -10,21 +10,21 @@ definition login :: "transition" where
         Guard = [],
         Outputs = [],
         Updates = [
-                    (R 1, (V (I 1))) (* Store the user ID in r1 *)
+                    (R 1, (V (I 1))) \<comment> \<open> Store the user ID in r1 \<close>
                   ]
       \<rparr>"
 
-(* Logs out the current user *)
+\<comment> \<open> Logs out the current user \<close>
 definition logout :: "transition" where
 "logout \<equiv> \<lparr>
         Label = ''logout'',
         Arity = 0,
-        Guard = [], (* No guards *)
+        Guard = [], \<comment> \<open> No guards \<close>
         Outputs = [],
-        Updates = [ (* Two updates: *)
-                    (R 1, (V (R 1))), (* Value of r1 remains unchanged *)
-                    (R 2, (V (R 2))), (* Value of r2 remains unchanged *)
-                    (R 3, (V (R 3)))  (* Value of r3 remains unchanged *)
+        Updates = [ \<comment> \<open> Two updates: \<close>
+                    (R 1, (V (R 1))), \<comment> \<open> Value of r1 remains unchanged \<close>
+                    (R 2, (V (R 2))), \<comment> \<open> Value of r2 remains unchanged \<close>
+                    (R 3, (V (R 3)))  \<comment> \<open> Value of r3 remains unchanged \<close>
                   ]
       \<rparr>"
 
@@ -32,12 +32,12 @@ definition "write" :: "transition" where
 "write \<equiv> \<lparr>
         Label = ''write'',
         Arity = 1,
-        Guard = [], (* No guards *)
+        Guard = [], \<comment> \<open> No guards \<close>
         Outputs = [],
         Updates = [
-                    (R 1, (V (R 1))), (* Value of r1 remains unchanged *)
-                    (R 2, (V (I 1))), (* Write the input to r2 *)
-                    (R 3, (V (R 1)))  (* Store the writer in r3 *)
+                    (R 1, (V (R 1))), \<comment> \<open> Value of r1 remains unchanged \<close>
+                    (R 2, (V (I 1))), \<comment> \<open> Write the input to r2 \<close>
+                    (R 3, (V (R 1)))  \<comment> \<open> Store the writer in r3 \<close>
                   ]
       \<rparr>"
 
@@ -45,7 +45,7 @@ definition "write_fail" :: "transition" where
 "write_fail \<equiv> \<lparr>
         Label = ''write'',
         Arity = 1,
-        Guard = [(Ne (V (R 3)) (V (R 1)))], (* No guards *)
+        Guard = [(Ne (V (R 3)) (V (R 1)))], \<comment> \<open> No guards \<close>
         Outputs = [(L (Str ''accessDenied''))],
         Updates = []
       \<rparr>"
@@ -54,12 +54,12 @@ definition read_success :: "transition" where
 "read_success \<equiv> \<lparr>
         Label = ''read'',
         Arity = 0,
-        Guard = [gexp.Eq (V (R 1)) (V (R 3)), (gNot (Null (R 2)))], (* No guards *)
+        Guard = [gexp.Eq (V (R 1)) (V (R 3)), (gNot (Null (R 2)))], \<comment> \<open> No guards \<close>
         Outputs = [(V (R 2))],
-        Updates = [ (* Two updates: *)
-                    (R 1, (V (R 1))), (* Value of r1 remains unchanged *)
-                    (R 2, (V (R 2))), (* Value of r2 remains unchanged *)
-                    (R 3, (V (R 3)))  (* Value of r3 remains unchanged *)
+        Updates = [ \<comment> \<open> Two updates: \<close>
+                    (R 1, (V (R 1))), \<comment> \<open> Value of r1 remains unchanged \<close>
+                    (R 2, (V (R 2))), \<comment> \<open> Value of r2 remains unchanged \<close>
+                    (R 3, (V (R 3)))  \<comment> \<open> Value of r3 remains unchanged \<close>
                   ]
       \<rparr>"
 
@@ -70,13 +70,19 @@ definition read_fail :: "transition" where
         Guard = [(gOr (Ne (V (R 1)) (V (R 3))) (Null (R 2)))],
         Outputs = [(L (Str ''accessDenied''))],
         Updates = [
-                    (R 1, (V (R 1))), (* Value of r1 remains unchanged *)
-                    (R 2, (V (R 2))), (* Value of r2 remains unchanged *)
-                    (R 3, (V (R 3)))  (* Value of r3 remains unchanged *)
+                    (R 1, (V (R 1))), \<comment> \<open> Value of r1 remains unchanged \<close>
+                    (R 2, (V (R 2))), \<comment> \<open> Value of r2 remains unchanged \<close>
+                    (R 3, (V (R 3)))  \<comment> \<open> Value of r3 remains unchanged \<close>
                   ]
       \<rparr>"
 
 datatype statename = q1 | q2
+
+lemma UNIV_statename: "UNIV = {q1 , q2}"
+  using statename.exhaust by auto
+
+instance statename :: finite
+  by standard (simp add: UNIV_statename)
 
 definition filesystem :: "statename efsm" where
 "filesystem \<equiv> \<lparr>
@@ -98,7 +104,7 @@ code_printing
   | constant False \<rightharpoonup> (Scala) "false"
   | constant HOL.conj \<rightharpoonup> (Scala) "_ && _"
 
-(* export_code GExp.satisfiable in "Scala" *)
+\<comment> \<open> export_code GExp.satisfiable in "Scala" \<close>
 
 value "(Contexts.apply_guard \<lbrakk>V (R 1) \<mapsto> Bc True, V (R 2) \<mapsto> Bc True\<rbrakk> ((gexp.Eq (V (R 2)) (L (Num 100))) \<or> (Ne (V (R 1)) (L (Num 100))))) (V (R 2))"
 
@@ -108,16 +114,16 @@ primrec all :: "'a list \<Rightarrow> ('a \<Rightarrow> bool) \<Rightarrow> bool
   "all [] _ = True" |
   "all (h#t) f = (if f h then all t f else False)"
 
-(* step :: efsm \<Rightarrow> statename \<Rightarrow> registers \<Rightarrow> label \<Rightarrow> inputs \<Rightarrow> (statename \<times> outputs \<times> registers) option *)
-(* observe_trace :: "efsm \<Rightarrow> statename \<Rightarrow> registers \<Rightarrow> trace \<Rightarrow> observation" where *)
+\<comment> \<open> step :: efsm \<Rightarrow> statename \<Rightarrow> registers \<Rightarrow> label \<Rightarrow> inputs \<Rightarrow> (statename \<times> outputs \<times> registers) option \<close>
+\<comment> \<open> observe_trace :: "efsm \<Rightarrow> statename \<Rightarrow> registers \<Rightarrow> trace \<Rightarrow> observation" where \<close>
 
-(* noChangeOwner: THEOREM filesystem |- G(cfstate /= NULL_STATE) => FORALL (owner : UID): G((label=write AND r_1=owner) => F(G((label=read AND r_1/=owner) => X(op_1_read_0 = accessDenied)))); *)
+\<comment> \<open> noChangeOwner: THEOREM filesystem |- G(cfstate /= NULL_STATE) => FORALL (owner : UID): G((label=write AND r_1=owner) => F(G((label=read AND r_1/=owner) => X(op_1_read_0 = accessDenied)))); \<close>
 
 lemma r_equals_r [simp]: "<R 1:=user, R 2:=content, R 3:=owner> = (\<lambda>a. if a = R 3 then Some owner else if a = R 2 then Some content else if a = R 1 then Some user else None)"
   apply (rule ext)
   by simp
 
-(* This one takes longer than you think to prove *)
+\<comment> \<open> This one takes longer than you think to prove \<close>
 lemma label_read_q2: "b \<in> T filesystem (q2, a) \<Longrightarrow> Label b = ''read'' \<Longrightarrow> a = q2 \<and> (b = read_success \<or> b = read_fail)"
   apply (simp add: filesystem_def)
   apply (cases a)
